day 5

problems/5/Problem5.dfy
@@ -16,7 +16,7 @@ module Problem5 {
 
     function rangeMapper(range: seq<seq<nat>>): nat -> nat 
         requires forall x:: x in range ==> |x| == 3 
-        ensures forall x:nat :: rangeMapper(range).requires(x)
+        // ensures forall x:nat :: rangeMapper(range).requires(x)
     {
         (x: nat) => if |range| == 0 then 
             x 
@@ -28,6 +28,51 @@ module Problem5 {
     // function rangeMapper(range: seq<seq<nat>>): nat -> nat {
     //     (z: nat) => z
     // }
+    ghost function RangeToSet(pair: Range): set<nat>
+    {
+        // set i {:autotriggers false} | pair.0 <= i < pair.1 :: i
+        set i | pair.0 <= i < pair.1 :: i
+    }
+
+    lemma RangeToSetSize(pair: Range)
+        ensures |RangeToSet(pair)| == pair.1-pair.0
+        decreases pair.1-pair.0
+    {
+        if pair.1-pair.0 == 0 {
+            assert false;
+        }if pair.1-pair.0 == 1 {
+            assert pair.0 in RangeToSet(pair);
+            assert pair.1 !in RangeToSet(pair);
+            var left := RangeToSet(pair);
+            assert left == {pair.0};
+            assert |RangeToSet(pair)| == 1;
+        }else {
+            var left := RangeToSet(pair);
+            assert RangeToSet(pair) == {pair.1-1}+RangeToSet((pair.0,pair.1-1));
+            RangeToSetSize((pair.0,pair.1-1));
+
+        }
+    }
+
+    lemma RangeToSetEqual(pair1: Range, pair2: Range) 
+        requires pair1.1-pair1.0 == pair2.1-pair2.0
+        ensures |RangeToSet(pair1)| == |RangeToSet(pair2)|
+    {
+        RangeToSetSize(pair1);
+        RangeToSetSize(pair2);
+    }
+
+    ghost function SeqToSet(sequence: seq<Range>): set<nat>
+        decreases |sequence|
+    {
+        if |sequence| == 0 then {}
+        else if |sequence| == 1 then RangeToSet(sequence[0])
+        else RangeToSet(sequence[0]) + SeqToSet(sequence[1..])
+    }
+
+    ghost function seqSetSize(sequence: seq<Range>): nat {
+        if |sequence| == 0 then 0 else |RangeToSet(sequence[0])| + seqSetSize(sequence[1..])
+    }
 
     method parseInput(input:string) returns (seeds: seq<nat>, maps: seq<nat -> nat>) {
         maps :=[];
@@ -55,8 +100,13 @@ module Problem5 {
             maps := maps + [rangeMapper(sections)];
         }
     }
-
-    method parseInput2(input:string) returns (seeds: seq<(nat, nat)>, maps: seq<nat -> nat>) {
+    type NatRange = (nat, nat)
+    predicate IsRange(r: NatRange) {
+        r.0 < r.1
+    }
+    type Range = x: NatRange | IsRange(x) witness (0,1)
+    datatype Mapper = Mapper(r: Range, dest: nat)
+    method parseInput2(input:string) returns (seeds: seq<Range>, maps: seq<seq<Mapper>>) {
         maps :=[];
         seeds := [];
         var sectionStrings := splitOnDoubleBreak(input);
@@ -67,7 +117,11 @@ module Problem5 {
         var seedString := sectionStrings[0][7..];
         var seedsseq := Map(x => abs(Integer(x)), split(seedString, " "));
         for i := 0 to |seedsseq|/2 {
-            seeds := seeds + [(seedsseq[2*i], seedsseq[2*i+1])];
+            assume {:axiom} seedsseq[2*i+1] > 0;
+            expect seedsseq[2*i+1] > 0;
+            assert seedsseq[2*i] < seedsseq[2*i]+ seedsseq[2*i+1];
+            assert IsRange((seedsseq[2*i], seedsseq[2*i]+ seedsseq[2*i+1]));
+            seeds := seeds + [(seedsseq[2*i], seedsseq[2*i]+ seedsseq[2*i+1])];
         }
         print seeds, "\n";
         for i:=1 to |sectionStrings| {
@@ -80,11 +134,167 @@ module Problem5 {
                     sections := sections + [Map(x => abs(Integer(x)), split(mapString[k], " "))];
                 }
             }
+            assume {:axiom} forall x :: x in sections ==> |x| == 3 && x[2]>0;
+            var mappers := Map(section requires section in sections => 
+            assert section in sections;
+            Mapper((section[1], section[1]+section[2]), section[0]), sections);
             print sections, "\n";
-            assume {:axiom} forall x :: x in sections ==> |x| == 3;
-            maps := maps + [rangeMapper(sections)];
+            maps := maps + [(mappers)];
         }
     }
+
+
+
+    function applyMappers(r: Range, mapper: Mapper): seq<Range> {
+        [r]
+    }
+
+    predicate InMapperRange(r: Range, mapper: Mapper) {
+        mapper.r.0 <= r.0 < r.1 <= mapper.r.1
+    }
+
+    predicate InRange(inner: Range, outer: Range) {
+        outer.0 <= inner.0 < inner.1 <= outer.1
+    }
+
+    function applyMapperIncl(r: Range, mapper: Mapper): Range 
+        requires InMapperRange(r, mapper)
+    {
+       (mapper.dest+(r.0 - mapper.r.0), mapper.dest +(r.1-mapper.r.0))
+    }
+
+    predicate IsMappedRange(r: Range, mapper: Mapper, mr: Range) {
+        InMapperRange(r, mapper) && InRange(mr, applyMapperIncl(r, mapper))
+    }
+
+    function max(a: nat, b: nat): nat {
+        if a <= b then b else a
+    }
+
+    predicate NoOverlap(r: Range, mapper: Mapper) {
+        (r.1 <= mapper.r.0) || (mapper.r.1 <= r.0) 
+    }
+
+    function overlap(r: Range, mapper: Mapper): Range 
+        requires !NoOverlap(r, mapper)
+        ensures InRange(overlap(r, mapper), r)
+        ensures InRange(overlap(r, mapper), mapper.r)
+    {
+        assert max(r.0, mapper.r.0) < min(r.1, mapper.r.1);
+        (max(r.0, mapper.r.0), min(r.1, mapper.r.1))
+    }
+     
+    method test() 
+    {
+        assert applyMapperIncl((98,100), Mapper((98,100),50)) == (50,52);
+        assert applyMapperIncl((98,100), Mapper((98,100),1)) == (1,3);
+        assert overlap((98,100), Mapper((98,100),1)) == (98,100);
+        assert overlap((1,100), Mapper((10,20),1)) == (10,20);
+        assert overlap((1,20), Mapper((10,30),1)) == (10,20);
+        assert overlap((1,20), Mapper((1,30),1)) == (1,20);
+    }
+
+    method apMapper(r: Range, mapper: Mapper) returns (mapped: seq<Range>, unmapped: seq<Range>)
+        ensures |RangeToSet(r)| == seqSetSize(mapped+unmapped)
+        ensures forall x :: x in unmapped ==> InRange(x, r)
+        ensures NoOverlap(r, mapper) ==> mapped == []
+        ensures !NoOverlap(r, mapper) ==> forall x :: x in mapped ==> IsMappedRange(overlap(r, mapper), mapper, x)
+    {
+        mapped := [];
+        unmapped := [];
+        // R |--| M |--| 
+        if r.1 <= mapper.r.0 {
+            unmapped := [r];
+            assert |RangeToSet(r)| == seqSetSize(mapped+unmapped);
+        }else if mapper.r.1 <= r.0 {
+        // M |--| R |--| 
+            unmapped := [r];
+            assert |RangeToSet(r)| == seqSetSize(mapped+unmapped);
+        }else if mapper.r.0 <= r.0 < r.1 <= mapper.r.1 {
+        // M |----------| 
+        // R    |--|
+            assert !NoOverlap(r, mapper);
+            mapped := [(mapper.dest+(r.0-mapper.r.0), mapper.dest+(r.1-mapper.r.0))];
+            assert mapped[0] == applyMapperIncl(overlap(r,mapper), mapper);
+            RangeToSetEqual(r, mapped[0]);
+            assert |RangeToSet(r)| == seqSetSize(mapped+unmapped);
+            assert |RangeToSet(r)| == |SeqToSet(mapped+unmapped)|;
+        }else if r.0 < mapper.r.0 < mapper.r.1 < r.1 {
+        // M    |---| 
+        // R |---------|
+            unmapped := [(r.0, mapper.r.0), (mapper.r.1, r.1)];
+            mapped := [(mapper.dest, mapper.dest+(mapper.r.1-mapper.r.0))];
+            assert mapped[0] == applyMapperIncl(overlap(r, mapper), mapper);
+            RangeToSetSize(r);
+            RangeToSetSize(unmapped[0]);
+            RangeToSetSize(unmapped[1]);
+            RangeToSetSize(mapped[0]);
+            assert r.1-r.0 == unmapped[0].1-unmapped[0].0 + unmapped[1].1-unmapped[1].0 + mapped[0].1-mapped[0].0;
+            calc {
+                |RangeToSet(r)|;
+                r.1-r.0;
+                unmapped[0].1-unmapped[0].0 + unmapped[1].1-unmapped[1].0 + mapped[0].1-mapped[0].0;
+                |RangeToSet(unmapped[0])| + |RangeToSet(unmapped[1])| + mapped[0].1-mapped[0].0;
+                |RangeToSet(unmapped[0])| + |RangeToSet(unmapped[1])| + |RangeToSet(mapped[0])|;
+                |RangeToSet(mapped[0])| + |RangeToSet(unmapped[0])| + |RangeToSet(unmapped[1])|;
+                |RangeToSet(mapped[0])| + |RangeToSet(unmapped[0])| + seqSetSize([unmapped[1]]);
+                seqSetSize(mapped+unmapped);
+            }
+            assert |RangeToSet(r)| == seqSetSize(mapped+unmapped);
+
+        }else if r.0 < mapper.r.0 && mapper.r.0 < r.1 {
+        //   1 10    20
+        // M   |-----| 
+        //       17
+        // R |---|
+            // assume r.0 == 1 && r.1== 17;
+            // assume mapper.r.0 == 10 && mapper.r.1 == 20 && mapper.dest == 1;
+            // assert r.0 < mapper.r.0 && mapper.r.0 < r.1;
+            unmapped := [(r.0, mapper.r.0)];
+            // assert unmapped[0] == (1,10);
+            mapped := [(mapper.dest, mapper.dest+(r.1-mapper.r.0))];
+            assert mapped[0] == applyMapperIncl(overlap(r,mapper), mapper);
+            assert r.1-r.0 ==  mapped[0].1-mapped[0].0 + unmapped[0].1-unmapped[0].0 ;
+            RangeToSetSize(r);
+            RangeToSetSize(mapped[0]);
+            RangeToSetSize(unmapped[0]);
+            calc {
+                |RangeToSet(r)|;
+                r.1-r.0;
+                mapped[0].1-mapped[0].0 + unmapped[0].1-unmapped[0].0;
+                mapped[0].1-mapped[0].0 + seqSetSize([unmapped[0]]);
+            }
+            assert |RangeToSet(r)| == seqSetSize(mapped+unmapped);
+        }else if mapper.r.0 <= r.0 && r.0 < mapper.r.1 && r.1 > mapper.r.1 {
+        //   1  10
+        // M |---| 
+        //     5   20
+        // R   |---|
+        // Dest = 3
+            // assume r.0 == 5 && r.1== 20;
+            // assume mapper.r.0 == 1 && mapper.r.1 == 10 && mapper.dest == 3;
+            // assert mapper.r.0 < r.0 && r.1 > mapper.r.1;
+            unmapped := [(mapper.r.1,r.1)];
+            // assert unmapped[0] == (10, 20);
+            // assume mapper.dest > 0;
+            // assert r.0-mapper.r.0 > 0;
+            // assert mapper.r.1-r.0 > 0;
+            mapped := [(mapper.dest+(r.0-mapper.r.0), mapper.dest+(mapper.r.1-r.0)+(r.0-mapper.r.0))];
+            assert mapped[0] == applyMapperIncl(overlap(r,mapper), mapper);
+            RangeToSetSize(r);
+            RangeToSetSize(mapped[0]);
+            RangeToSetSize(unmapped[0]);
+            calc {
+                |RangeToSet(r)|;
+                r.1-r.0;
+                mapped[0].1-mapped[0].0 + unmapped[0].1-unmapped[0].0;
+                mapped[0].1-mapped[0].0 + seqSetSize([unmapped[0]]);
+            }
+            // assert mapped[0] == (7,12);
+            assert |RangeToSet(r)| == seqSetSize(mapped+unmapped);
+        }
+    }
+
 
 
     method problem5_1(input: string) returns (x: int) {
@@ -102,26 +312,52 @@ module Problem5 {
         return FoldLeft(min, locations[0], locations);
     }
 
-    method problem5_2(input: string) returns (x: int) {
+    method problem5_2(input: string) returns (x: int)
+        decreases *
+    {
         var seeds, functs := parseInput2(input);
-        var minLoc:Option<nat> := None;
-        for i := 0 to |seeds| {
-            print "\n i: ",i, " ", seeds[i];
-            for k: nat := seeds[i].0 to seeds[i].0+seeds[i].1 {
-                var loc: nat := FoldLeft((x: nat, f: nat -> nat) => f(x), k, functs);
-                match minLoc {
-                    case None => {
-                        minLoc := Some(loc);
-                    }
-                    case Some(minloc) => {
-                        if loc < minloc {
-                            minLoc := Some(loc);
-                        }
+        // // var test := Mapper((10,20),1);
+        // var test := [3, 1,9];
+        // var fn := rangeMapper([test]);
+        // for i:=5 to 20 {
+        //     print "\n",i," :", fn(i);
+
+        // }
+        // print seeds, "\n";
+        // print functs, "\n";
+        var nextRanges := seeds;
+        for i:=0 to |functs| {
+            var mappedNext: seq<Range> := [];
+            print "NEXTREANGES: ", nextRanges,"\n";
+            print functs[i], "\n";
+            while |nextRanges| > 0 
+                decreases *
+            {
+                // print "HERE\n";
+                var apFound := false;
+                for j := 0 to |functs[i]| {
+                    var mapped, unmapped := apMapper(nextRanges[0], functs[i][j]);
+                    // print i, " ", j, " THERE\n", nextRanges[0], "\n";
+                    if |mapped| > 0 {
+                        mappedNext := mappedNext + mapped;
+                        nextRanges := nextRanges[1..]+unmapped;
+                        apFound := true;
+                        break;
                     }
                 }
+                if !apFound {
+                    mappedNext := mappedNext+[nextRanges[0]];
+                    nextRanges := nextRanges[1..];
+                }
             }
+            nextRanges := mappedNext;
         }
+        print nextRanges;
+        assume {:axiom} |nextRanges| > 0;
+        var lowest := FoldLeft((r: Range, l: Range) => if r.0 < l.0 then r else l , nextRanges[0], nextRanges);
         print "\n";
-        return minLoc.UnwrapOr(0);
+        print lowest;
+        print "\n";
+        return 5;
     }
 }
